formalization/EquivRedProperties.v
@@ -1,0 +1,523 @@
+From FD Require Import Syntax.
+From FD Require Import Reduction.
+From FD Require Import FreeVars.
+From FD Require Import Renaming.
+From FD Require Import FreeVars.
+From FD Require Import StructCong.
+From FD Require Import Contexts.
+From FD Require Import Typing.
+From FD Require Import Preservation.
+From FD Require Import ConfluenceDefs.
+From FD Require Import DirectedCong.
+From FD Require Import AxCutCtx.
+From FD Require Import ParallelReduction.
+
+From Stdlib Require Import Lia.
+
+(******************************************************************************)
+(* up_subst_n                                                                 *)
+(******************************************************************************)
+(* Definition for up_subst_n is in DirectedCongruence.v *)
+(* Here are some more helpful lemmata about it *)
+
+Lemma up_subst_Sn :
+  forall j σ, up_subst (up_subst_n j σ) = up_subst_n (S j) σ.
+Proof. auto. Qed.
+
+Lemma substitutions_compose :
+  (forall P σ1 σ2,
+    subst_process (subst_process P σ1) σ2
+      = subst_process P (fun x => subst_message (σ1 x) σ2)) /\
+  (forall M σ1 σ2,
+    subst_message (subst_message M σ1) σ2
+      = subst_message M (fun x => subst_message (σ1 x) σ2)) /\
+  (forall s σ1 σ2,
+    subst_statement (subst_statement s σ1) σ2
+      = subst_statement s (fun x => subst_message (σ1 x) σ2)).
+Proof.
+  apply syntax_ind; intros; simpl;
+  try assert (
+    forall x,
+      (fun x : nat => subst_message (up_subst σ1 x) (up_subst σ2)) x
+       = (up_subst (fun x : nat => subst_message (σ1 x) σ2)) x
+  ) by (
+    intros [|]; auto; simpl;
+    replace (up_subst σ2) with (up_subst_n 1 σ2) by auto;
+    unfold upM; rewrite (proj1 (proj2 subst_up_lift_commute)); auto
+  );
+  try rewrite H; try rewrite H0; auto; f_equal; apply subst_extensional; auto.
+  intros [|[|]]; auto; simpl. unfold upM.
+  replace (up_subst (up_subst σ2)) with (up_subst_n 1 (up_subst σ2)) by auto.
+  rewrite (proj1 (proj2 subst_up_lift_commute)); simpl.
+  replace (up_subst σ2) with (up_subst_n 1 σ2) by auto.
+  rewrite (proj1 (proj2 subst_up_lift_commute)).
+  auto.
+Qed.
+
+Lemma up_subst_n_additive :
+  forall n1 n2 σ,
+    up_subst_n n1 (up_subst_n n2 σ) = up_subst_n (n1 + n2) σ.
+Proof.
+  induction n1; intros; simpl; auto. rewrite IHn1. auto.
+Qed.
+
+Lemma well_formedness_under_up_subst :
+  forall E j n σ,
+    well_formed_axcut_ctx j E ->
+    j < n ->
+    well_formed_axcut_ctx j (subst_ctx E (up_subst_n n σ)).
+Proof.
+  induction E; intros; auto; simpl; econstructor;
+  replace (up_subst (up_subst_n n σ)) with (up_subst_n (S n) σ) by auto.
+  + eapply nfv_under_substitution_extensional; intros.
+    destruct (Compare_dec.lt_dec n0 (S n)).
+    - rewrite up_subst_n_lt; auto.
+      intro. inversion H2; subst. inversion H. congruence.
+    - rewrite up_subst_n_ge; try lia.
+      apply nfv_lift_n. lia.
+  + apply IHE; try lia. inversion H; auto.
+  + eapply nfv_under_substitution_extensional; intros.
+    destruct (Compare_dec.lt_dec n0 (S n)).
+    - rewrite up_subst_n_lt; auto.
+      intro. inversion H2; subst. inversion H. congruence.
+    - rewrite up_subst_n_ge; try lia.
+      apply nfv_lift_n. lia.
+  + apply IHE; try lia. inversion H; auto.
+Qed.
+
+Lemma down_after_lift_Sk_lift_k :
+  (forall P, forall n1 n2 k, n1 <= n2 -> n2 <= n1 + k ->
+    down1_process (lift_process P n1 (S k)) n2 = lift_process P n1 k)
+  /\
+  (forall M, forall n1 n2 k, n1 <= n2 -> n2 <= n1 + k ->
+    down1_message (lift_message M n1 (S k)) n2 = lift_message M n1 k)
+  /\
+  (forall s, forall n1 n2 k, n1 <= n2 -> n2 <= n1 + k ->
+    down1_statement (lift_statement s n1 (S k)) n2 = lift_statement s n1 k).
+Proof.
+  apply syntax_ind; intros; simpl; auto;
+  try (now (rewrite H; try rewrite H0; auto; try lia)).
+  unfold relocate.
+  destruct (Nat.leb n1 n) eqn:E.
+  + apply PeanoNat.Nat.leb_le in E.
+    assert (n2 < (S k + n)) by lia.
+    apply PeanoNat.Nat.ltb_lt in H1; rewrite H1; auto.
+  + apply PeanoNat.Nat.leb_nle in E.
+    assert (~ n2 < n) by lia.
+    apply PeanoNat.Nat.ltb_nlt in H1; rewrite H1; auto.
+Qed.
+
+Lemma up_subst_down_commute :
+  (forall P, forall σ k j,
+    ~ (j ∈ P) -> j <= k ->
+    down1_process (subst_process P (up_subst_n (S k) σ)) j =
+    subst_process (down1_process P j) (up_subst_n k σ)) /\
+  (forall M, forall σ k j,
+    ~ (occurs_free_message j M) -> j <= k ->
+    down1_message (subst_message M (up_subst_n (S k) σ)) j =
+    subst_message (down1_message M j) (up_subst_n k σ)) /\
+  (forall s, forall σ k j,
+    ~ (occurs_free_statement j s) -> j <= k ->
+    down1_statement (subst_statement s (up_subst_n (S k) σ)) j =
+    subst_statement (down1_statement s j) (up_subst_n k σ)).
+Proof.
+  apply syntax_ind; intros; simpl;
+  try replace (up_subst (up_subst_n k σ)) with (up_subst_n (S k) σ) by auto;
+  try replace (up_subst (up_subst_n (S k) σ)) with (up_subst_n (S (S k)) σ) by auto;
+  try (now (try rewrite H; try rewrite H0; auto; try lia; intro Hfv; try apply H1; try apply H0; free_var_econstructor; eauto)).
+  + assert (j <> n). { intro. apply H; subst. free_var_econstructor; eauto. }
+    destruct (Nat.ltb j n) eqn:E.
+    - apply PeanoNat.Nat.ltb_lt in E. destruct n; try (exfalso; lia); simpl.
+      destruct (Nat.ltb n k) eqn:E1.
+      * apply PeanoNat.Nat.ltb_lt in E1.
+        rewrite up_subst_n_lt; auto; simpl.
+        unfold relocate; simpl. apply PeanoNat.Nat.ltb_lt in E; rewrite E.
+        auto.
+      * apply PeanoNat.Nat.ltb_nlt in E1.
+        rewrite up_subst_n_ge; try lia.
+        unfold upM.
+        rewrite (proj1 (proj2 shift_additive)).
+        rewrite PeanoNat.Nat.add_1_r.
+        rewrite (proj1 (proj2 down_after_lift_Sk_lift_k)); auto. lia.
+    - apply PeanoNat.Nat.ltb_nlt in E.
+      rewrite up_subst_n_lt; try lia; simpl.
+      apply PeanoNat.Nat.ltb_nlt in E; rewrite E.
+      rewrite up_subst_n_lt; auto.
+      apply PeanoNat.Nat.ltb_nlt in E; lia.
+  + replace (up_subst (up_subst_n (S (S k)) σ)) with (up_subst_n (S (S (S k))) σ) by auto.
+    rewrite H; auto. intro Hfv. apply H0. free_var_econstructor. auto. lia.
+Qed.
+
+Lemma up_subst_lift_commute :
+  (forall P, forall σ k j,
+    j <= k ->
+    lift_process (subst_process P (up_subst_n k σ)) j 1 =
+    subst_process (lift_process P j 1) (up_subst_n (S k) σ)) /\
+  (forall M, forall σ k j,
+    j <= k ->
+    lift_message (subst_message M (up_subst_n k σ)) j 1 =
+    subst_message (lift_message M j 1) (up_subst_n (S k) σ)) /\
+  (forall s, forall σ k j,
+    j <= k ->
+    lift_statement (subst_statement s (up_subst_n k σ)) j 1 =
+    subst_statement (lift_statement s j 1) (up_subst_n (S k) σ)).
+Proof.
+  apply syntax_ind; intros; simpl;
+  try replace (up_subst (up_subst_n k σ)) with (up_subst_n (S k) σ) by auto;
+  try replace (up_subst (up_subst_n (S k) σ)) with (up_subst_n (S (S k)) σ) by auto;
+  try (now (try rewrite H; try rewrite H0; auto; try lia; intro Hfv; try apply H1; try apply H0; free_var_econstructor; eauto)).
+  destruct (Compare_dec.lt_dec n k).
+  - rewrite up_subst_n_lt; auto.
+    unfold relocate. destruct (Nat.leb j n) eqn:E; simpl.
+    * unfold relocate. rewrite E. rewrite up_subst_n_lt; auto.
+    * unfold relocate. rewrite E. rewrite up_subst_Sn.
+      rewrite up_subst_n_lt; auto.
+  - rewrite up_subst_n_ge; try lia.
+    unfold relocate.
+    assert (j <= n) by lia. apply PeanoNat.Nat.leb_le in H0; rewrite H0; simpl.
+    rewrite up_subst_n_ge; try lia. unfold upM.
+    rewrite (proj1 (proj2 shift_shift_raise_bound)); try lia; simpl.
+    rewrite (proj1 (proj2 shift_shift_raise_bound)) with (n2 := 0); try lia.
+    auto.
+Qed.
+
+(******************************************************************************)
+(* Substitution and evaluation contexts                                       *)
+(******************************************************************************)
+Lemma subst_ctx_preserves_length :
+  forall E σ,
+    length_axcut_ctx (subst_ctx E σ) = length_axcut_ctx E.
+Proof.
+  induction E; intros; simpl; auto.
+Qed.
+
+Lemma subst_over_fill_hole :
+  forall E M j σ,
+    well_formed_axcut_ctx j E ->
+    σ j = future j ->
+    subst_process (fill_hole E M) σ
+      = fill_hole (subst_ctx E σ) (subst_message M (up_subst_n (length_axcut_ctx E) σ)).
+Proof.
+  induction E; intros; simpl.
+  + inversion H; subst. rewrite H0; auto.
+  + inversion H; subst. rewrite H0; auto.
+  + f_equal. rewrite IHE with (j := S j).
+    - f_equal; f_equal.
+      replace (up_subst σ) with (up_subst_n 1 σ) by auto.
+      rewrite up_subst_n_additive. rewrite PeanoNat.Nat.add_1_r.
+      auto.
+    - inversion H; auto.
+    - simpl. rewrite H0. auto.
+  + f_equal. rewrite IHE with (j := S j).
+    - f_equal; f_equal.
+      replace (up_subst σ) with (up_subst_n 1 σ) by auto.
+      rewrite up_subst_n_additive. rewrite PeanoNat.Nat.add_1_r.
+      auto.
+    - inversion H; auto.
+    - simpl. rewrite H0. auto.
+Qed.
+
+Lemma ren_subst_ctx_commute :
+  forall E, forall r σ k,
+    bijective r -> (forall j, j >= k -> r j = j) ->
+    (forall j, j < k -> (σ j) = (future j)) ->
+    (forall j, j >= k -> (rename_message (σ j) r) = (σ j)) ->
+    subst_ctx (rename_axcut_ctx E r) σ
+      = rename_axcut_ctx (subst_ctx E σ) r.
+Proof.
+  induction E; intros; simpl; auto.
+  + assert (
+      forall j : nat, j >= (S k) -> up_ren r j = j
+    ).
+    { intros [|] ?; auto; simpl. rewrite H0; auto; lia. }
+    assert (
+      forall j : nat, j < S k -> up_subst σ j = future j
+    ).
+    {
+      intros [|] ?; auto; simpl. rewrite H1; simpl; auto; lia.
+    }
+    assert (
+      forall j : nat, j >= S k -> rename_message (up_subst σ j) (up_ren r) = up_subst σ j
+    ).
+    {
+      intros [|] ?; auto; simpl.
+      unfold upM.
+      rewrite (proj1 (proj2 ren_up_up_ren_commute)); auto.
+      + rewrite H2; auto; lia.
+      + intros; exfalso; lia.
+    }
+    assert (
+      bijective (up_ren r)
+    ) by (apply shift_preserves_bijection; auto).
+    erewrite IHE; eauto. erewrite (proj1 ren_subst_commute); eauto.
+  + assert (
+      forall j : nat, j >= (S k) -> up_ren r j = j
+    ).
+    { intros [|] ?; auto; simpl. rewrite H0; auto; lia. }
+    assert (
+      forall j : nat, j < S k -> up_subst σ j = future j
+    ).
+    {
+      intros [|] ?; auto; simpl. rewrite H1; simpl; auto; lia.
+    }
+    assert (
+      forall j : nat, j >= S k -> rename_message (up_subst σ j) (up_ren r) = up_subst σ j
+    ).
+    {
+      intros [|] ?; auto; simpl.
+      unfold upM.
+      rewrite (proj1 (proj2 ren_up_up_ren_commute)); auto.
+      + rewrite H2; auto; lia.
+      + intros; exfalso; lia.
+    }
+    assert (
+      bijective (up_ren r)
+    ) by (apply shift_preserves_bijection; auto).
+    erewrite IHE; eauto. erewrite (proj1 ren_subst_commute); eauto.
+Qed.
+
+Lemma up_subst_n_over_reduce_axcut' :
+  forall n E M P j σ,
+    n = length_axcut_ctx E ->
+    well_formed_axcut_ctx 0 E ->
+    ~ (occurs_free_message (length_axcut_ctx E) M) ->
+    subst_process (reduce_axcut E M P) (up_subst_n j σ) =
+    reduce_axcut
+      (subst_ctx E (up_subst_n (S j) σ))
+      (subst_message M (up_subst_n (length_axcut_ctx E + (S j)) σ))
+      (subst_process P (up_subst_n (S j) σ)).
+Proof.
+  induction n; intros; simpl;
+  destruct E; simpl in H; try congruence; simpl.
+  + repeat rewrite reduce_axcut_equation_1; simpl.
+    repeat rewrite (proj1 substitutions_compose).
+    apply subst_extensional.
+    intros [|]; simpl.
+    - replace (up_subst (up_subst_n j σ)) with (up_subst_n (S j) σ) by auto.
+      unfold downM.
+      rewrite (proj1 (proj2 up_subst_down_commute)); auto; try lia.
+    - rewrite (proj1 (proj2 subst_nfv_down)) with (n := 0).
+      * unfold upM. rewrite (proj1 (proj2 down_after_up_id)). auto.
+      * apply nfv_lift_n; lia.
+      * intros; exfalso; lia.
+      * intros; auto.
+  + repeat rewrite reduce_axcut_equation_2; simpl.
+    repeat rewrite (proj1 substitutions_compose).
+    apply subst_extensional.
+    intros [|]; simpl.
+    - replace (up_subst (up_subst_n j σ)) with (up_subst_n (S j) σ) by auto.
+      unfold downM.
+      rewrite (proj1 (proj2 up_subst_down_commute)); auto; try lia.
+    - rewrite (proj1 (proj2 subst_nfv_down)) with (n := 0).
+      * unfold upM. rewrite (proj1 (proj2 down_after_up_id)). auto.
+      * apply nfv_lift_n; lia.
+      * intros; exfalso; lia.
+      * intros; auto.
+  + repeat rewrite reduce_axcut_equation_3; simpl.
+    f_equal.
+    - repeat rewrite up_subst_Sn.
+      unfold down.
+      replace swap01 with (up_ren_n 0 swap01) by auto. inversion H0; subst.
+      repeat rewrite (proj1 up_ren_n_swap_down_down_Sn); auto.
+      * rewrite (proj1 up_subst_down_commute); auto. lia.
+      * apply nfv_under_substitution_extensional; intros.
+        destruct (Compare_dec.lt_dec n0 (S (S j))).
+        ** rewrite up_subst_n_lt; auto.
+           intro. inversion H3; subst. congruence.
+        ** rewrite up_subst_n_ge; try lia. apply nfv_lift_n. lia.
+    - replace (up_subst (up_subst_n j σ)) with (up_subst_n (S j) σ) by auto.
+      rewrite IHn.
+      * f_equal.
+        ** rewrite up_subst_Sn.
+           apply ren_subst_ctx_commute with (k := S (S j)); try apply swap01_is_bijective.
+           ++ intros [|[|]] ?; auto; exfalso; lia.
+           ++ intros. rewrite up_subst_n_lt; auto.
+           ++ intros. rewrite up_subst_n_ge; try lia.
+              rewrite (proj1 (proj2 renaming_idempotent_free_vars)); auto.
+              intros. destruct n0 as [|[|]]; auto; exfalso.
+              -- assert (
+                  ~ occurs_free_message 0 (lift_message (σ (j0 - S (S j))) 0 (S (S j)))
+                 ). { apply nfv_lift_n; lia. } congruence.
+              -- assert (
+                  ~ occurs_free_message 1 (lift_message (σ (j0 - S (S j))) 0 (S (S j)))
+                 ). { apply nfv_lift_n; lia. } congruence.
+        ** repeat rewrite up_subst_Sn.
+           rewrite <- rename_axcut_ctx_preserves_length.
+           replace (S (length_axcut_ctx E + S j)) with (length_axcut_ctx E + (S (S j))) by lia.
+           rewrite subst_ctx_preserves_length.
+           apply (proj1 (proj2 ren_subst_commute)) with (k := length_axcut_ctx E + S (S j)).
+           ++ apply up_ren_n_preserves_bijection; apply swap01_is_bijective.
+           ++ intros. rewrite up_ren_n_swap_not_nSn; lia.
+           ++ intros. rewrite up_subst_n_lt; auto.
+           ++ intros. rewrite up_subst_n_ge; try lia.
+              rewrite (proj1 (proj2 renaming_idempotent_free_vars)); auto.
+              intros. rewrite up_ren_n_swap_not_nSn; auto; intro; subst.
+              -- assert (
+                  ~ occurs_free_message (length_axcut_ctx E)
+                      (lift_message (σ (j0 - (length_axcut_ctx E + S (S j)))) 0 (length_axcut_ctx E + S (S j)))
+                 ). { apply nfv_lift_n; lia. } congruence.
+              -- assert (
+                  ~ occurs_free_message (S (length_axcut_ctx E))
+                      (lift_message (σ (j0 - (length_axcut_ctx E + S (S j)))) 0 (length_axcut_ctx E + S (S j)))
+                 ). { apply nfv_lift_n; lia. } congruence.
+        ** unfold up.
+           repeat rewrite (proj1 up_ren_n_swap_lift_lift_Sn).
+           rewrite (proj1 up_subst_lift_commute); auto. lia.
+      * rewrite <- rename_axcut_ctx_preserves_length; inversion H; auto.
+      * replace 0 with (swap01 1) by auto; replace swap01 with (up_ren_n 0 swap01) by auto.
+        apply well_formedness_preserved_under_swap01.
+        inversion H0; auto.
+      * rewrite <- rename_axcut_ctx_preserves_length.
+        replace (length_axcut_ctx E) with
+          (up_ren_n (length_axcut_ctx E) swap01 (S (length_axcut_ctx E)))
+          at 1 by (rewrite up_ren_n_swap_Sn; auto).
+        apply (proj1 (proj2 nfv_under_renaming)).
+        apply up_ren_n_preserves_bijection; apply swap01_is_bijective.
+        assumption.
+  + repeat rewrite reduce_axcut_equation_4; simpl.
+    f_equal.
+    - replace (up_subst (up_subst_n j σ)) with (up_subst_n (S j) σ) by auto.
+      rewrite IHn.
+      * f_equal.
+        ** rewrite up_subst_Sn.
+           apply ren_subst_ctx_commute with (k := S (S j)); try apply swap01_is_bijective.
+           ++ intros [|[|]] ?; auto; exfalso; lia.
+           ++ intros. rewrite up_subst_n_lt; auto.
+           ++ intros. rewrite up_subst_n_ge; try lia.
+              rewrite (proj1 (proj2 renaming_idempotent_free_vars)); auto.
+              intros. destruct n0 as [|[|]]; auto; exfalso.
+              -- assert (
+                  ~ occurs_free_message 0 (lift_message (σ (j0 - S (S j))) 0 (S (S j)))
+                 ). { apply nfv_lift_n; lia. } congruence.
+              -- assert (
+                  ~ occurs_free_message 1 (lift_message (σ (j0 - S (S j))) 0 (S (S j)))
+                 ). { apply nfv_lift_n; lia. } congruence.
+        ** repeat rewrite up_subst_Sn.
+           rewrite <- rename_axcut_ctx_preserves_length.
+           replace (S (length_axcut_ctx E + S j)) with (length_axcut_ctx E + (S (S j))) by lia.
+           rewrite subst_ctx_preserves_length.
+           apply (proj1 (proj2 ren_subst_commute)) with (k := length_axcut_ctx E + S (S j)).
+           ++ apply up_ren_n_preserves_bijection; apply swap01_is_bijective.
+           ++ intros. rewrite up_ren_n_swap_not_nSn; lia.
+           ++ intros. rewrite up_subst_n_lt; auto.
+           ++ intros. rewrite up_subst_n_ge; try lia.
+              rewrite (proj1 (proj2 renaming_idempotent_free_vars)); auto.
+              intros. rewrite up_ren_n_swap_not_nSn; auto; intro; subst.
+              -- assert (
+                  ~ occurs_free_message (length_axcut_ctx E)
+                      (lift_message (σ (j0 - (length_axcut_ctx E + S (S j)))) 0 (length_axcut_ctx E + S (S j)))
+                 ). { apply nfv_lift_n; lia. } congruence.
+              -- assert (
+                  ~ occurs_free_message (S (length_axcut_ctx E))
+                      (lift_message (σ (j0 - (length_axcut_ctx E + S (S j)))) 0 (length_axcut_ctx E + S (S j)))
+                 ). { apply nfv_lift_n; lia. } congruence.
+        ** unfold up.
+           repeat rewrite (proj1 up_ren_n_swap_lift_lift_Sn).
+           rewrite (proj1 up_subst_lift_commute); auto. lia.
+      * rewrite <- rename_axcut_ctx_preserves_length; inversion H; auto.
+      * replace 0 with (swap01 1) by auto; replace swap01 with (up_ren_n 0 swap01) by auto.
+        apply well_formedness_preserved_under_swap01.
+        inversion H0; auto.
+      * rewrite <- rename_axcut_ctx_preserves_length.
+        replace (length_axcut_ctx E) with
+          (up_ren_n (length_axcut_ctx E) swap01 (S (length_axcut_ctx E)))
+          at 1 by (rewrite up_ren_n_swap_Sn; auto).
+        apply (proj1 (proj2 nfv_under_renaming)).
+        apply up_ren_n_preserves_bijection; apply swap01_is_bijective.
+        assumption.
+    - repeat rewrite up_subst_Sn.
+      unfold down.
+      replace swap01 with (up_ren_n 0 swap01) by auto. inversion H0; subst.
+      repeat rewrite (proj1 up_ren_n_swap_down_down_Sn); auto.
+      * rewrite (proj1 up_subst_down_commute); auto. lia.
+      * apply nfv_under_substitution_extensional; intros.
+        destruct (Compare_dec.lt_dec n0 (S (S j))).
+        ** rewrite up_subst_n_lt; auto.
+           intro. inversion H3; subst. congruence.
+        ** rewrite up_subst_n_ge; try lia. apply nfv_lift_n. lia.
+Qed.
+
+Lemma up_subst_n_over_reduce_axcut :
+  forall E M P j σ,
+    well_formed_axcut_ctx 0 E ->
+    ~ (occurs_free_message (length_axcut_ctx E) M) ->
+    subst_process (reduce_axcut E M P) (up_subst_n j σ) =
+    reduce_axcut
+      (subst_ctx E (up_subst_n (S j) σ))
+      (subst_message M (up_subst_n (length_axcut_ctx E + (S j)) σ))
+      (subst_process P (up_subst_n (S j) σ)).
+Proof.
+  intros; eapply up_subst_n_over_reduce_axcut'; auto.
+Qed.
+
+(******************************************************************************)
+(* Lemmata for Confluence                                                     *)
+(******************************************************************************)
+Lemma equiv_red_invariant_under_substitution :
+  forall Γ P P' σ, Γ ⊢ P :# -> P ⊵ P' ->
+    (subst_process P σ) ⊵ (subst_process P' σ).
+Proof.
+  intros.
+  generalize dependent σ.
+  generalize dependent Γ.
+  induction H0; intros; simpl;
+  try (now econstructor).
+  + econstructor. rewrite H. unfold up.
+    repeat rewrite (proj1 up_ren_n_swap_lift_lift_Sn).
+    replace (up_subst σ) with (up_subst_n 1 σ) by auto.
+    rewrite <- (proj1 subst_up_lift_commute).
+    reflexivity.
+  + econstructor. rewrite H. unfold up.
+    repeat rewrite (proj1 up_ren_n_swap_lift_lift_Sn).
+    replace (up_subst σ) with (up_subst_n 1 σ) by auto.
+    rewrite <- (proj1 subst_up_lift_commute).
+    reflexivity.
+  + rewrite H. rewrite subst_over_fill_hole with (j := 0); auto.
+    rewrite H1. replace σ with (up_subst_n 0 σ) at 4 by auto.
+    rewrite up_subst_n_over_reduce_axcut; auto; simpl.
+    - assert (
+        up_subst_n (length_axcut_ctx E) (up_subst σ)
+          = up_subst_n (length_axcut_ctx E + 1) σ
+      ).
+      { replace (up_subst σ) with (up_subst_n 1 σ) by auto. rewrite up_subst_n_additive. auto. }
+      rewrite H3.
+      eapply rp_ax_cut_l; eauto.
+      replace (up_subst σ) with (up_subst_n 1 σ) by auto.
+      apply well_formedness_under_up_subst; auto.
+    - inversion H2; subst.
+      replace (length_axcut_ctx E) with (length_axcut_ctx E + 0) by lia.
+      apply (nfv_well_typed_fill_hole _ _ _ _ H0 H7).
+  + rewrite H. rewrite subst_over_fill_hole with (j := 0); auto.
+    rewrite H1. replace σ with (up_subst_n 0 σ) at 4 by auto.
+    rewrite up_subst_n_over_reduce_axcut; auto; simpl.
+    - assert (
+        up_subst_n (length_axcut_ctx E) (up_subst σ)
+          = up_subst_n (length_axcut_ctx E + 1) σ
+      ).
+      { replace (up_subst σ) with (up_subst_n 1 σ) by auto. rewrite up_subst_n_additive. auto. }
+      rewrite H3.
+      eapply rp_ax_cut_r; eauto.
+      replace (up_subst σ) with (up_subst_n 1 σ) by auto.
+      apply well_formedness_under_up_subst; auto.
+    - inversion H2; subst.
+      replace (length_axcut_ctx E) with (length_axcut_ctx E + 0) by lia.
+      apply (nfv_well_typed_fill_hole _ _ _ _ H0 H8).
+  + assert (
+      subst_process (subst_process P (prefix s ⋅ id_subst)) σ
+        = subst_process (subst_process P (up_subst σ)) (prefix (subst_statement s σ) ⋅ id_subst)
+    ).
+    {
+      repeat rewrite (proj1 substitutions_compose).
+      apply subst_extensional.
+      intros [|]; auto; simpl.
+      rewrite (proj1 (proj2 subst_nfv_down)) with (n := 0).
+      + unfold upM. rewrite (proj1 (proj2 down_after_up_id)); auto.
+      + apply nfv_lift_n; lia.
+      + intros; exfalso; lia.
+      + auto.
+    }
+    rewrite H0. econstructor.
+  + apply rp_cong_cut_l. inversion H; subst. eapply IHequiv_reduces; eauto.
+  + apply rp_cong_cut_r. inversion H; subst. eapply IHequiv_reduces; eauto.
+  + apply rp_cong_seq. inversion H; subst. eapply IHequiv_reduces; eauto.
+Qed.
